LeanNanoLlvm/Semantics.lean
@@ -1,4 +1,4 @@
 import LeanNanoLlvm.Semantics.Semantics
 import LeanNanoLlvm.Semantics.State
-import LeanNanoLlvm.Semantics.Denote
+import LeanNanoLlvm.Semantics.Eval
 import LeanNanoLlvm.Semantics.Wellformed
