LeanNanoLlvm/Tactic.lean
@@ -3,4 +3,4 @@ import Lean.Meta.Tactic.Simp.RegisterCommand
 register_simp_attr simp_llvm
 register_simp_attr simp_llvm_option
 register_simp_attr simp_wellform
-register_simp_attr simp_denote
+register_simp_attr simp_eval
